Proof of refinement triple for lock free read. Still need to update recovery proof.
The abstraction relation had to be updated to account for the fact that readers
may have to do a form of helping in the simulation proof.  Consider a scenario
where a write finishes the write to d0, and is then paused. Suppose then that
d1 fails. A read begins and first reads d1, finding that it has failed, so it
will then read and return the value in d0. In other words, because d1 has
failed, the write has effectively already taken place, so its linearization
point needs to be before the read. Thus, in this case, the reader will first
simulate the step of the writer and then simulate its own read.

src/Examples/ReplicatedDisk/ReplicatedDiskImpl.v
@@ -30,6 +30,22 @@ Definition read (addr: nat) :=
    Ret v
    else (_ <- Ret tt; Ret 0))%proc.
 
+(* A lock free version of read. The idea is to read d1 first, before checking d0 *)
+
+Definition lock_free_read (addr: nat) :=
+  (if lt_dec addr size then
+   v <- (rd1 <- read_disk d1 addr;
+           match rd1 with
+           | Some v => Ret v
+           | None => rd0 <- read_disk d0 addr;
+             match rd0 with
+             | Some v => Ret v
+             | None => Ret 0
+             end
+           end);
+   Ret v
+   else (_ <- Ret tt; Ret 0))%proc.
+
 Definition fixup (a: addr) : proc Op unit :=
   (rd0 <- read_disk d0 a;
    match rd0 with
@@ -51,5 +67,13 @@ Definition impl : LayerImpl TwoDisk.Op OneDisk.Op :=
        match op with
        | OneDisk.Write_Disk a v => write a v
        | OneDisk.Read_Disk a => read a
+       end;
+     recover := Seq_Cons (recv) (Seq_Nil); |}.
+
+Definition lock_free_impl : LayerImpl TwoDisk.Op OneDisk.Op :=
+  {| compile_op T (op: OneDisk.Op T) :=
+       match op with
+       | OneDisk.Write_Disk a v => write a v
+       | OneDisk.Read_Disk a => lock_free_read a
        end;
      recover := Seq_Cons (recv) (Seq_Nil); |}.
